Update AbstractSimplicialComplex.lean

Coxeter/ForMathlib/AbstractSimplicialComplex.lean
@@ -47,6 +47,9 @@ instance : SetLike (AbstractSimplicialComplex V) (Finset V) where
 theorem mem_faces {F : AbstractSimplicialComplex V} {x : Finset V} : x ∈ F.faces ↔ x ∈ F :=
   Iff.rfl
 
+lemma eq_iff_faces (F G : AbstractSimplicialComplex V) : F = G ↔ F.faces = G.faces := by
+  constructor <;> (intro h; ext; rw [h])
+
 @[simp]
 def le (G F : AbstractSimplicialComplex V) := G.faces ⊆ F.faces
 
@@ -142,30 +145,22 @@ lemma sup_faces (F G : AbstractSimplicialComplex V) : (F ⊔ G).faces = F.faces 
   rw [show F ⊔ G = sSup s by simp [s], show F.faces ∪ G.faces = ⋃ i : s, i.1.faces by simp [s], sSup_faces_of_nonempty (by simp [s])]
 
 @[simp]
-theorem iInf_faces {ι : Type*} (x : ι → AbstractSimplicialComplex V) : (⨅ i, x i).faces = ⨅ i, (x i).faces := by --might be wrong
-  sorry
+theorem iInf_faces {ι : Type*} (x : ι → AbstractSimplicialComplex V) : (⨅ i, x i).faces = ⋂ i, (x i).faces := by
+  unfold iInf
+  simp only [sInf_def, Set.iInter_coe_set, Set.mem_range, Set.iInter_exists, Set.iInter_iInter_eq',
+    Set.sInf_eq_sInter, Set.sInter_range]
 
 @[simp]
-theorem iSup_faces {ι : Type*} (x : ι → AbstractSimplicialComplex V) : (⨆ i, x i).faces = ⨆ i, (x i).faces := by
-  sorry
+theorem iSup_faces_of_nonempty {ι : Type*} (x : ι → AbstractSimplicialComplex V) [Nonempty ι] : (⨆ i, x i).faces = ⋃ i, (x i).faces := by
+  unfold iSup
+  rw [sSup_faces_of_nonempty]
+  · simp
+  · by_contra h
+    apply Set.not_nonempty_iff_eq_empty.1 at h
+    simp at h
 
-/--
-Definition: For any ASC F, we denote by vertices F the set of vertices of F.
--/
+/-- Definition: For any ASC `F`, we denote by `vertices F` the set of vertices of F. -/
 def vertices (F : AbstractSimplicialComplex V) : Set V := ⋃ s : F.faces, s.1.toSet
-
-lemma vertices_iff_singleton_set_face (F : AbstractSimplicialComplex V) (x : V) :
-    {x} ∈ F.faces ↔ x ∈ vertices F := by
-  constructor
-  · intro hx
-    simp only [vertices, Set.iUnion_coe_set, mem_faces,
-      Set.mem_iUnion, Finset.mem_coe, exists_prop]
-    exact ⟨{x}, And.intro hx (Finset.mem_singleton.mpr rfl)⟩
-  · rintro ⟨sx, ⟨⟨a, ha⟩, hxsx⟩⟩
-    rw [← ha] at hxsx
-    refine @lower' V F a.1 _ ?_ a.2
-    simp only [Finset.le_eq_subset, Finset.singleton_subset_iff]
-    exact hxsx
 
 /--
 Definition: Let `F` be an ASC. A maximal face of F is called a facet of F.
@@ -207,16 +202,13 @@ lemma isPure_iff_isPure' {F : AbstractSimplicialComplex V} : F.IsPure ↔ ∃ d,
       use d
     · intro
       simp only [nonempty_subtype, not_exists] at hemp
-      intro s hs t _
+      intro s hs
       exfalso
       exact hemp s hs
 
 lemma pure_def {F : AbstractSimplicialComplex V} [Pure F] : ∀ s ∈ F.Facets, ∀ t ∈ F.Facets, s.card = t.card := Pure.pure
 
 lemma pure_isPure {F : AbstractSimplicialComplex V} [Pure F] : IsPure F := pure_def
-
-theorem isPure_iSup {ι : Type*} {p : ι → AbstractSimplicialComplex V} (hp : ∀i : ι, IsPure (p i)) : IsPure (⨆ i : ι, p i) := by
-  sorry
 
 /--
 The rank of an ASC is defined to be the supremum of the cardinals of its faces.
@@ -230,6 +222,8 @@ noncomputable def rank (F : AbstractSimplicialComplex V) : ℕ := iSup fun s : F
 as faces.
 
 Remark: Here we secretly consider the ambient space as the simplex with vertex set V.
+
+Maybe don't use `abbrev` will be better? Because sometimes we don't want `simp` to expand this construction.
 -/
 abbrev closure (s : Set (Finset V))
   : AbstractSimplicialComplex V := sInf {K | s ⊆  K.faces}
@@ -239,7 +233,9 @@ lemma subset_closure_faces (s : Set (Finset V)) : s ⊆ (closure s).faces := by
     imp_self, forall_const]
 
 lemma closure_faces_eq_self (F : AbstractSimplicialComplex V) : closure F.faces = F := by
-  sorry
+  apply le_antisymm
+  · apply sInf_le; simp; rfl
+  · simp
 
 lemma closure_mono {s t: Set (Finset V)} : s ⊆ t → closure s ≤ closure t := by
   intro hst
@@ -247,18 +243,14 @@ lemma closure_mono {s t: Set (Finset V)} : s ⊆ t → closure s ≤ closure t :
   rw [Set.setOf_subset_setOf]
   intro _ h; exact Set.Subset.trans hst h
 
-/--
-Lemma: For a `f : Finset V`, the closure of `{f}` is the simplex of `f`.
--/
+/-- Lemma: For a `f : Finset V`, the closure of `{f}` is the simplex of `f`.-/
 lemma closure_simplex (f : Finset V) : closure {f} =  simplex f := by
   have h1 : (closure {f}).faces = (simplex f).faces:= by
-    apply Set.Subset.antisymm
-    · rw [sInf_def]
-      rintro s h1
+    apply Set.Subset.antisymm <;> rw [sInf_def]
+    · rintro s h1
       simp only [Set.singleton_subset_iff, mem_faces, Set.mem_setOf_eq, Set.mem_iInter, Set.coe_setOf, Subtype.forall] at h1
       exact h1 (simplex ↑f) fun ⦃_⦄ a => a
-    · rw [sInf_def]
-      rintro s h1
+    · rintro s h1
       apply simplex_face.1 at h1
       simp only [Finset.coe_subset] at h1
       simp only [Set.singleton_subset_iff, mem_faces, Set.mem_setOf_eq, Set.mem_iInter, Set.coe_setOf, Subtype.forall]
@@ -270,7 +262,7 @@ lemma closure_simplex (f : Finset V) : closure {f} =  simplex f := by
 def closurePower (s : Set (Finset V)) : AbstractSimplicialComplex V where
   faces :=
     if Nonempty s then
-      ⋃ f : s, {t | t.toSet ⊆ f}
+      ⋃ f : s, {t | t ⊆ f}
     else
       {∅}
   empty_mem := by
@@ -279,8 +271,7 @@ def closurePower (s : Set (Finset V)) : AbstractSimplicialComplex V where
   lower' := by
     by_cases h : Nonempty s <;> simp [h]
     · refine isLowerSet_iUnion₂ ?_
-      intro t _
-      intro a b h1 h2
+      intro t _ a b h1 h2
       refine' Set.Subset.trans ?_ h2
       congr
     · exact Finset.isLowerSet_singleton_empty V
@@ -310,14 +301,13 @@ lemma closure_eq_iSup (s : Set (Finset V)) : closure s = ⨆ f : s,  closure {f.
 
 theorem closure_eq_closurePower (s: Set (Finset V)) : closure s = closurePower s := by
   ext t
-  constructor
-  · intro ts
-    rw[closure] at ts
-    simp at ts
+  constructor <;> intro ts
+  · simp only [sInf_def, Set.coe_setOf, Set.mem_setOf_eq, Set.mem_iInter, mem_faces,
+    Subtype.forall] at ts
     unfold closurePower
     apply ts
     by_cases h : Nonempty s <;> simp [h]
-    · rw[Set.subset_def]
+    · rw [Set.subset_def]
       intro x xs
       simp only [Set.mem_iUnion, Set.mem_setOf_eq, exists_prop]
       use x
@@ -326,21 +316,31 @@ theorem closure_eq_closurePower (s: Set (Finset V)) : closure s = closurePower s
       intro g hg
       rw [h] at hg
       contradiction
-  · intro ts
-    rw[closurePower] at ts
+  · rw [closurePower] at ts
     by_cases h : Nonempty s <;> simp [h]
     · simp [closurePower,h] at ts
       intro K sK
       obtain ⟨f,fs⟩ := ts
-      rw[Set.subset_def] at sK
+      rw [Set.subset_def] at sK
       obtain ⟨fs, tf⟩ := fs
       apply sK at fs
       exact mem_faces.1 <| K.lower' tf <| fs
-    · simp [closurePower,h] at ts
+    · simp [closurePower, h] at ts
       intro K _
       apply mem_faces.1
       rw [ts]
       exact K.empty_mem
+
+lemma closure_faces (s : Set (Finset V)) : (closure s).faces = if Nonempty s then ⋃ f : s, {t : Finset V | t ⊆ f} else {∅} := by
+  rw [closure_eq_closurePower]; rfl
+
+lemma closure_singleton_faces (f : Finset V) : (closure {f}).faces = {t : Finset V | t ⊆ f} := by
+  rw [closure_faces]
+  simp only [nonempty_subtype, Set.mem_singleton_iff, exists_eq, ↓reduceIte, Set.iUnion_coe_set,
+    Set.iUnion_iUnion_eq_left]
+
+-- lemma closure_singleton_faces' (f : Finset V) : (closure {f}).faces = Finset.powerset f := by
+--   rw [closure_singleton_faces]
 
 instance instNonemptyToAbstractSimplicialComplexContainingSet (s : Set (Finset V)) : Nonempty {x : AbstractSimplicialComplex V // s ⊆ x.faces} := ⟨closure s, subset_closure_faces _⟩
 
@@ -372,17 +372,59 @@ instance instCompleteDistribLatticeToAbstractSimplicialComplex : CompleteDistrib
       intro i is f hf
       rw [Set.mem_iUnion]
       use i
-      simp [is, hf]
-    · simp [Set.not_nonempty_iff_eq_empty.mp hs]
+      simp only [is, iSup_pos, inf_faces, hf]
+    · simp only [Set.not_nonempty_iff_eq_empty.mp hs, sSup_empty, ge_iff_le, bot_le,
+      inf_of_le_right, Set.mem_empty_iff_false, not_false_eq_true, iSup_neg, iSup_bot, le_refl]
   iInf_sup_le_sup_sInf := by
     intro a s
-    simp [Set.union_iInter]
+    simp only [le_def, iInf_faces, sup_faces, sInf_def, Set.iInter_coe_set, Set.union_iInter,
+      Set.subset_iInter_iff]
     intro i is f hf
     rw [Set.mem_iInter] at hf
     replace hf := hf i
-    simp [is] at hf
-    simp [hf]
+    simp only [is, iInf_pos, sup_faces, Set.mem_union, mem_faces] at hf
+    simp only [Set.mem_union, mem_faces, hf]
 }
+
+@[simp]
+theorem closure_singleton_Facets (f : Finset V) : (closure {f}).Facets = {f} := by
+  ext g; constructor <;> intro hg
+  · rcases hg with ⟨hg_mem, hg_max⟩
+    rw [Set.mem_singleton_iff]
+    contrapose! hg_max
+    use f; constructor
+    · apply mem_faces.mp
+      apply Set.mem_of_subset_of_mem <| subset_closure_faces {f}
+      rfl
+    · refine ⟨?_, hg_max⟩
+      rw [← mem_faces, closure_faces] at hg_mem
+      simpa only [nonempty_subtype, Set.mem_singleton_iff, exists_eq, ↓reduceIte,
+        Set.iUnion_coe_set, Set.iUnion_iUnion_eq_left, Set.mem_setOf_eq] using hg_mem
+  · rw [Set.mem_singleton_iff] at hg
+    subst hg; constructor
+    · apply Set.mem_of_subset_of_mem <| subset_closure_faces {g}; rfl
+    · intro t ht
+      rw [← mem_faces, closure_faces] at ht
+      simp only [nonempty_subtype, Set.mem_singleton_iff, exists_eq, ↓reduceIte, Set.iUnion_coe_set,
+        Set.iUnion_iUnion_eq_left, Set.mem_setOf_eq] at ht
+      apply fun h ↦ subset_antisymm h ht
+
+
+theorem isPure_closure_singelton (f : Finset V) : IsPure (closure {f}) := by
+  intro s hs t ht
+  rw [closure_singleton_Facets, Set.mem_singleton_iff] at *
+  rw [hs, ht]
+
+theorem closure_singleton_inter_eq_inf {f g : Finset V} : closure {f ∩ g} = closure {f} ⊓ closure {g} := by
+  simp only [eq_iff_faces, inf_faces, closure_singleton_faces]
+  ext x; constructor <;> {
+    intro h
+    simpa only [Set.mem_inter_iff, Set.mem_setOf_eq, Finset.subset_inter_iff] using h
+  }
+
+theorem isPure_inf_closure_singleton {f g : Finset V} : IsPure (closure {f} ⊓ closure {g}) := by
+  rw [← closure_singleton_inter_eq_inf]
+  apply isPure_closure_singelton
 
 lemma bot_eq_ofEmpty' : (⊥ : AbstractSimplicialComplex V) = closurePower ∅ := by
   symm
@@ -391,13 +433,59 @@ lemma bot_eq_ofEmpty' : (⊥ : AbstractSimplicialComplex V) = closurePower ∅ :
 
 lemma bot_eq_ofEmpty : (⊥ : AbstractSimplicialComplex V) = closure ∅ := by
   symm
-  rw[closure_eq_closurePower]
+  rw [closure_eq_closurePower]
   rw [eq_bot_iff, le_def, show (closurePower ∅).faces = {∅} by simp[closurePower], Set.singleton_subset_iff]
   apply (⊥ : AbstractSimplicialComplex V).empty_mem
 
 @[simp]
 lemma bot_faces_eq_empty : (⊥ : AbstractSimplicialComplex V).faces = {∅} := by
   rw [bot_eq_ofEmpty']
-  simp[closurePower]
+  simp only [closurePower, nonempty_subtype, Set.mem_empty_iff_false, exists_const, ↓reduceIte]
+
+@[simp]
+theorem bot_Facets : (⊥ : AbstractSimplicialComplex V).Facets = {∅} := by
+  ext x; constructor <;> intro hx
+  · rw [← bot_faces_eq_empty, mem_faces]
+    exact hx.1
+  · rw [Set.mem_singleton_iff.mp hx]
+    refine ⟨(⊥ : AbstractSimplicialComplex V).empty_mem, ?_⟩
+    intro t ht _
+    rw [← mem_faces, bot_faces_eq_empty, Set.mem_singleton_iff] at ht
+    exact ht.symm
+
+@[simp]
+theorem isPure_bot : IsPure (⊥ : AbstractSimplicialComplex V) := by
+  intro s hs t ht
+  rw [bot_Facets, Set.mem_singleton_iff] at *
+  rw [hs, ht]
+
+@[simp]
+theorem iSup_faces_of_isEmpty {ι : Type*} [IsEmpty ι] (x : ι → AbstractSimplicialComplex V) : (⨆ i, x i).faces = {∅} := by
+  simp only [iSup_of_empty, bot_faces_eq_empty]
+
+theorem iSup_Facets_le_of_nonempty {ι : Type*} [Nonempty ι] {p : ι → AbstractSimplicialComplex V} : (⨆ i : ι, p i).Facets ≤ ⋃ i : ι, (p i).Facets := by
+  intro a ha
+  rw [Set.mem_iUnion]
+  rcases ha with ⟨ha_mem, ha_max⟩
+  rw [← mem_faces, iSup_faces_of_nonempty, Set.mem_iUnion] at ha_mem
+  rcases ha_mem with ⟨i, hi⟩
+  use i
+  constructor
+  · exact mem_faces.mpr hi
+  · intro t ht
+    apply ha_max
+    rw [← mem_faces, iSup_faces_of_nonempty]
+    apply Set.mem_iUnion_of_mem i ht
+
+@[deprecated]
+theorem isPure_iSup {ι : Type*} {p : ι → AbstractSimplicialComplex V} {d : ℕ} (hp : ∀i : ι, IsPure' (p i) d) : IsPure' (⨆ i : ι, p i) d := by
+  by_cases hemp : Nonempty ι
+  · sorry
+  · rw [not_nonempty_iff] at hemp
+    rw [iSup_of_empty]
+    sorry
+
+
+
 
 end AbstractSimplicialComplex
